hax-lib/core-models/alloc/src/lib.rs
@@ -285,6 +285,26 @@ pub mod vec {
             seq_concat(&mut self.0, &other.0);
             other.0 = seq_empty()
         }
+        #[hax_lib::opaque]
+        pub fn drain<R /* : RangeBounds<usize> */>(&mut self, _range: R) -> drain::Drain<T, A> {
+            drain::Drain(seq_slice(&self.0, 0, self.len()), std::marker::PhantomData::<A>) // TODO use range bounds
+        }
+    }
+    pub mod drain {
+        use rust_primitives::sequence::*;
+        pub struct Drain<T, A>(pub Seq<T>, pub std::marker::PhantomData<A>);
+        impl<T, A> Iterator for Drain<T, A> {
+            type Item = T;
+            fn next(&mut self) -> Option<Self::Item> {
+            if seq_len(&self.0) == 0 {
+                Option::None
+            } else {
+                let res = seq_first(&self.0);
+                self.0 = seq_slice(&self.0, 1, seq_len(&self.0));
+                Option::Some(res)
+            }
+        }
+        }
     }
 
     #[hax_lib::attributes]
