hax-lib/core-models/src/core/array.rs
@@ -1,3 +1,5 @@
+use rust_primitives::{sequence::*, slice::*};
+
 pub struct TryFromSliceError;
 
 // Dummy type to allow impls
@@ -31,13 +33,38 @@ impl<T> Dummy<T, 0> {}
 
 impl<T, const N: usize> Dummy<T, N> {
     pub fn map<U>(s: [T; N], f: fn(T) -> U) -> [U; N] {
-        rust_primitives::slice::array_map(s, f)
+        array_map(s, f)
     }
     pub fn as_slice(s: [T; N]) -> &'static [T] {
-        rust_primitives::slice::array_as_slice(s)
+        array_as_slice(s)
     }
 }
 
 pub fn from_fn<T, const N: usize>(f: fn(usize) -> T) -> [T; N] {
-    rust_primitives::slice::array_from_fn(f)
+    array_from_fn(f)
+}
+
+impl<T, const N: usize> crate::iter::traits::collect::IntoIterator for [T; N] {
+    type IntoIter = iter::IntoIter<T, N>;
+    fn into_iter(self) -> iter::IntoIter<T, N> {
+        iter::IntoIter(seq_from_array(self))
+    }
+}
+
+mod iter {
+    use crate::option::Option;
+    use rust_primitives::sequence::*;
+    pub struct IntoIter<T, const N: usize>(pub Seq<T>);
+    impl<T, const N: usize> crate::iter::traits::iterator::Iterator for IntoIter<T, N> {
+        type Item = T;
+        fn next(&mut self) -> Option<T> {
+            if seq_len(&self.0) == 0 {
+                Option::None
+            } else {
+                let res = seq_first(&self.0);
+                self.0 = seq_slice(&self.0, 1, seq_len(&self.0));
+                Option::Some(res)
+            }
+        }
+    }
 }
