hax-lib/core-models/src/core/iter.rs
@@ -1,0 +1,303 @@
+// This model of iterators doesn't respect the signatures of the original definitions in Rust core.
+// We avoid default implementations for trait methods, and instead provide them as external to the trait.
+// This means overriding them is not possible.
+// We also avoid the coinductivity between `IntoIter` and `Iterator`.
+
+pub mod traits {
+    pub mod iterator {
+        use super::super::adapters::{
+            enumerate::Enumerate, flat_map::FlatMap, flatten::Flatten, map::Map, step_by::StepBy,
+            take::Take, zip::Zip,
+        };
+        use crate::ops::function::*;
+        use crate::option::Option;
+        #[hax_lib::attributes]
+        pub trait Iterator {
+            type Item;
+            #[hax_lib::requires(true)]
+            fn next(&mut self) -> Option<Self::Item>;
+        }
+        #[hax_lib::opaque]
+        fn fold<I: Iterator, B, F: FnOnce<(B, I::Item), Output = B>>(
+            mut it: I,
+            init: B,
+            f: F,
+        ) -> B {
+            let mut accum = init;
+            while let Option::Some(x) = it.next() {
+                accum = f.call_once((accum, x));
+            }
+            accum
+        }
+
+        fn enumerate<I: Iterator>(it: I) -> Enumerate<I> {
+            Enumerate::new(it)
+        }
+
+        fn step_by<I: Iterator>(it: I, step: usize) -> StepBy<I> {
+            StepBy::new(it, step)
+        }
+
+        fn map<I: Iterator, O, F: FnOnce<I::Item, Output = O>>(it: I, f: F) -> Map<I, F> {
+            Map::new(it, f)
+        }
+
+        #[hax_lib::opaque]
+        fn all<I: Iterator, F: FnOnce<I::Item, Output = bool>>(mut it: I, f: F) -> bool {
+            while let Option::Some(x) = it.next() {
+                if !f.call_once(x) {
+                    return false;
+                }
+            }
+            true
+        }
+
+        fn take<I: Iterator>(it: I, n: usize) -> Take<I> {
+            Take::new(it, n)
+        }
+
+        fn flat_map<I: Iterator, U: Iterator, F: FnOnce<I::Item, Output = U>>(
+            it: I,
+            f: F,
+        ) -> FlatMap<I, U, F> {
+            FlatMap::new(it, f)
+        }
+
+        fn flatten<I: Iterator>(it: I) -> Flatten<I>
+        where
+            I::Item: Iterator,
+        {
+            Flatten::new(it)
+        }
+
+        fn zip<I1: Iterator, I2: Iterator>(it1: I1, it2: I2) -> Zip<I1, I2> {
+            Zip::new(it1, it2)
+        }
+
+        // TODO rev: DoubleEndedIterator?
+    }
+    pub mod collect {
+        pub trait IntoIterator {
+            // Ignoring type Item, and trait bound Iterator to avoid coinduction
+            // type Item;
+            type IntoIter; //: Iterator<Item = Self::Item>
+            fn into_iter(self) -> Self::IntoIter;
+        }
+    }
+}
+
+pub mod adapters {
+    pub mod enumerate {
+        use super::super::traits::iterator::Iterator;
+        use crate::option::Option;
+        pub struct Enumerate<I> {
+            iter: I,
+            count: usize,
+        }
+        impl<I> Enumerate<I> {
+            pub fn new(iter: I) -> Enumerate<I> {
+                Enumerate { iter, count: 0 }
+            }
+        }
+        impl<I: Iterator> Iterator for Enumerate<I> {
+            type Item = (usize, <I as Iterator>::Item);
+
+            fn next(&mut self) -> Option<(usize, <I as Iterator>::Item)> {
+                match self.iter.next() {
+                    Option::Some(a) => {
+                        let i = self.count;
+                        // TODO check what to do here. It would be bad to have an iterator with 
+                        // more than usize::MAX elements, this could be a requirement (but hard to formulate).
+                        hax_lib::assume!(self.count < usize::MAX); 
+                        self.count += 1;
+                        Option::Some((i, a))
+                    }
+                    Option::None => Option::None,
+                }
+            }
+        }
+    }
+    pub mod step_by {
+        use super::super::traits::iterator::Iterator;
+        use crate::option::Option;
+        pub struct StepBy<I> {
+            iter: I,
+            step: usize,
+        }
+        impl<I> StepBy<I> {
+            pub fn new(iter: I, step: usize) -> Self {
+                StepBy { iter, step }
+            }
+        }
+
+        #[hax_lib::opaque]
+        impl<I: Iterator> Iterator for StepBy<I> {
+            type Item = <I as Iterator>::Item;
+
+            fn next(&mut self) -> Option<<I as Iterator>::Item> {
+                for _ in 1..self.step {
+                    if let Option::None = self.iter.next() {
+                        return Option::None;
+                    }
+                }
+                self.iter.next()
+            }
+        }
+    }
+    pub mod map {
+        pub struct Map<I, F> {
+            iter: I,
+            f: F,
+        }
+        impl<I, F> Map<I, F> {
+            pub fn new(iter: I, f: F) -> Self {
+                Self { iter, f }
+            }
+        }
+        use super::super::traits::iterator::Iterator;
+        use crate::ops::function::*;
+        use crate::option::Option;
+        impl<I: Iterator, O, F: FnOnce<I::Item, Output = O>> Iterator for Map<I, F> {
+            type Item = O;
+
+            fn next(&mut self) -> Option<O> {
+                match self.iter.next() {
+                    Option::Some(v) => Option::Some(self.f.call_once(v)),
+                    Option::None => Option::None,
+                }
+            }
+        }
+    }
+    pub mod take {
+        use super::super::traits::iterator::Iterator;
+        use crate::option::Option;
+        pub struct Take<I> {
+            iter: I,
+            n: usize,
+        }
+        impl<I> Take<I> {
+            pub fn new(iter: I, n: usize) -> Take<I> {
+                Take { iter, n }
+            }
+        }
+        impl<I: Iterator> Iterator for Take<I> {
+            type Item = <I as Iterator>::Item;
+
+            fn next(&mut self) -> Option<<I as Iterator>::Item> {
+                if self.n != 0 {
+                    self.n -= 1;
+                    self.iter.next()
+                } else {
+                    Option::None
+                }
+            }
+        }
+    }
+    pub mod flat_map {
+        use super::super::traits::iterator::Iterator;
+        use crate::option::Option;
+        pub struct FlatMap<I, U, F> {
+            it: I,
+            f: F,
+            current: Option<U>,
+        }
+        impl<I: Iterator, U: Iterator, F: FnOnce<I::Item, Output = U>> FlatMap<I, U, F> {
+            pub fn new(it: I, f: F) -> Self {
+                Self {
+                    it,
+                    f,
+                    current: Option::None,
+                }
+            }
+        }
+        use crate::ops::function::*;
+        #[hax_lib::opaque]
+        impl<I: Iterator, U: Iterator, F: FnOnce<I::Item, Output = U>> Iterator for FlatMap<I, U, F> {
+            type Item = U::Item;
+            fn next(&mut self) -> Option<U::Item> {
+                loop {
+                    if let Option::Some(current_it) = &mut self.current
+                        && let Option::Some(v) = current_it.next()
+                    {
+                        return Option::Some(v);
+                    } else {
+                        match self.it.next() {
+                            Option::Some(c) => self.current = Option::Some(self.f.call_once(c)),
+                            Option::None => return Option::None,
+                        }
+                    }
+                }
+            }
+        }
+    }
+    pub mod flatten {
+        use super::super::traits::iterator::Iterator;
+        use crate::option::Option;
+        #[hax_lib::fstar::before("noeq")] // https://github.com/cryspen/hax/issues/1810
+        pub struct Flatten<I: Iterator> 
+        where
+            I::Item: Iterator,
+        {
+            it: I,
+            current: Option<I::Item>,
+        }
+        impl<I: Iterator> Flatten<I>
+        where
+            I::Item: Iterator,
+        {
+            pub fn new(it: I) -> Self {
+                Self {
+                    it,
+                    current: Option::None,
+                }
+            }
+        }
+        #[hax_lib::opaque]
+        impl<I: Iterator> Iterator for Flatten<I>
+        where
+            I::Item: Iterator,
+        {
+            type Item = <<I as Iterator>::Item as Iterator>::Item;
+            fn next(&mut self) -> Option<<<I as Iterator>::Item as Iterator>::Item> {
+                loop {
+                    if let Option::Some(current_it) = &mut self.current
+                        && let Option::Some(v) = current_it.next()
+                    {
+                        return Option::Some(v);
+                    } else {
+                        match self.it.next() {
+                            Option::Some(c) => self.current = Option::Some(c),
+                            Option::None => return Option::None,
+                        }
+                    }
+                }
+            }
+        }
+    }
+    pub mod zip {
+        use super::super::traits::iterator::Iterator;
+        use crate::option::Option;
+        pub struct Zip<I1, I2> {
+            it1: I1,
+            it2: I2,
+        }
+        impl<I1: Iterator, I2: Iterator> Zip<I1, I2> {
+            pub fn new(it1: I1, it2: I2) -> Self {
+                Self { it1, it2 }
+            }
+        }
+        #[hax_lib::opaque]
+        impl<I1: Iterator, I2: Iterator> Iterator for Zip<I1, I2> {
+            type Item = (I1::Item, I2::Item);
+            fn next(&mut self) -> Option<Self::Item> {
+                match self.it1.next() {
+                    Option::Some(v1) => match self.it2.next() {
+                        Option::Some(v2) => Option::Some((v1, v2)),
+                        Option::None => Option::None,
+                    },
+                    Option::None => Option::None,
+                }
+            }
+        }
+    }
+}
