hax-lib/proof-libs/fstar/core/Core_models.Slice.Iter.fst
@@ -1,8 +1,50 @@
 module Core_models.Slice.Iter
-
+#set-options "--fuel 0 --ifuel 1 --z3rlimit 15"
+open FStar.Mul
 open Rust_primitives
 
-unfold let t_Chunks a = t_Slice (t_Slice a)
-unfold let t_ChunksExact a = t_Slice (t_Slice a)
-unfold let t_Iter a = t_Slice a
+type t_Chunks (v_T: Type0) = | Chunks : Rust_primitives.Sequence.t_Seq v_T -> t_Chunks v_T
 
+type t_ChunksExact (v_T: Type0) =
+  | ChunksExact : Rust_primitives.Sequence.t_Seq v_T -> t_ChunksExact v_T
+
+type t_Iter (v_T: Type0) = | Iter : Rust_primitives.Sequence.t_Seq v_T -> t_Iter v_T
+
+[@@ FStar.Tactics.Typeclasses.tcinstance]
+let impl (#v_T: Type0) : Core_models.Iter.Traits.Iterator.t_Iterator (t_Iter v_T) =
+  {
+    f_Item = v_T;
+    f_next_pre = (fun (self: t_Iter v_T) -> true);
+    f_next_post
+    =
+    (fun (self: t_Iter v_T) (out: (t_Iter v_T & Core_models.Option.t_Option v_T)) -> true);
+    f_next
+    =
+    fun (self: t_Iter v_T) ->
+      let (self: t_Iter v_T), (hax_temp_output: Core_models.Option.t_Option v_T) =
+        if (Rust_primitives.Sequence.seq_len #v_T self._0 <: usize) =. mk_usize 0
+        then
+          self, (Core_models.Option.Option_None <: Core_models.Option.t_Option v_T)
+          <:
+          (t_Iter v_T & Core_models.Option.t_Option v_T)
+        else
+          let res:v_T = Rust_primitives.Sequence.seq_first #v_T self._0 in
+          let self:t_Iter v_T =
+            {
+              self with
+              _0
+              =
+              Rust_primitives.Sequence.seq_slice #v_T
+                self._0
+                (mk_usize 1)
+                (Rust_primitives.Sequence.seq_len #v_T self._0 <: usize)
+            }
+            <:
+            t_Iter v_T
+          in
+          self, (Core_models.Option.Option_Some res <: Core_models.Option.t_Option v_T)
+          <:
+          (t_Iter v_T & Core_models.Option.t_Option v_T)
+      in
+      self, hax_temp_output <: (t_Iter v_T & Core_models.Option.t_Option v_T)
+  }
