hax-lib/proof-libs/fstar/core/Alloc.Alloc.fst
@@ -1,6 +1,6 @@
 module Alloc.Alloc
 #set-options "--fuel 0 --ifuel 1 --z3rlimit 15"
 open FStar.Mul
-open Core_models
+open Rust_primitives
 
 type t_Global = | Global : t_Global
