hax-lib/proof-libs/fstar/core/Alloc.Boxed.fst
@@ -1,7 +1,7 @@
 module Alloc.Boxed
 #set-options "--fuel 0 --ifuel 1 --z3rlimit 15"
 open FStar.Mul
-open Core_models
+open Rust_primitives
 
 type t_Box (v_T: Type0) (v_A: Type0) =
   | Box : v_T -> Core_models.Option.t_Option v_A -> t_Box v_T v_A
