hax-lib/proof-libs/fstar/core/Alloc.Fmt.fst
@@ -1,7 +1,7 @@
 module Alloc.Fmt
 #set-options "--fuel 0 --ifuel 1 --z3rlimit 15"
 open FStar.Mul
-open Core_models
+open Rust_primitives
 
 assume
 val format': args: Core_models.Fmt.t_Arguments -> Alloc.String.t_String
