hax-lib/proof-libs/fstar/core/Core_models.Iter.Bundle.fst
@@ -1,0 +1,377 @@
+module Core_models.Iter.Bundle
+#set-options "--fuel 0 --ifuel 1 --z3rlimit 15"
+open FStar.Mul
+open Rust_primitives
+
+type t_Enumerate (v_I: Type0) = {
+  f_iter:v_I;
+  f_count:usize
+}
+
+let impl__new (#v_I: Type0) (iter: v_I) : t_Enumerate v_I =
+  { f_iter = iter; f_count = mk_usize 0 } <: t_Enumerate v_I
+
+type t_FlatMap (v_I: Type0) (v_U: Type0) (v_F: Type0) = {
+  f_it:v_I;
+  f_f:v_F;
+  f_current:Core_models.Option.t_Option v_U
+}
+
+type t_Map (v_I: Type0) (v_F: Type0) = {
+  f_iter:v_I;
+  f_f:v_F
+}
+
+let impl__new__from__map (#v_I #v_F: Type0) (iter: v_I) (f: v_F) : t_Map v_I v_F =
+  { f_iter = iter; f_f = f } <: t_Map v_I v_F
+
+type t_StepBy (v_I: Type0) = {
+  f_iter:v_I;
+  f_step:usize
+}
+
+let impl__new__from__step_by (#v_I: Type0) (iter: v_I) (step: usize) : t_StepBy v_I =
+  { f_iter = iter; f_step = step } <: t_StepBy v_I
+
+type t_Take (v_I: Type0) = {
+  f_iter:v_I;
+  f_n:usize
+}
+
+let impl__new__from__take (#v_I: Type0) (iter: v_I) (n: usize) : t_Take v_I =
+  { f_iter = iter; f_n = n } <: t_Take v_I
+
+type t_Zip (v_I1: Type0) (v_I2: Type0) = {
+  f_it1:v_I1;
+  f_it2:v_I2
+}
+
+class t_Iterator (v_Self: Type0) = {
+  [@@@ FStar.Tactics.Typeclasses.no_method]f_Item:Type0;
+  f_next_pre:self_: v_Self -> pred: Type0{true ==> pred};
+  f_next_post:v_Self -> (v_Self & Core_models.Option.t_Option f_Item) -> Type0;
+  f_next:x0: v_Self
+    -> Prims.Pure (v_Self & Core_models.Option.t_Option f_Item)
+        (f_next_pre x0)
+        (fun result -> f_next_post x0 result)
+}
+
+[@@ FStar.Tactics.Typeclasses.tcinstance]
+let impl_1 (#v_I: Type0) (#[FStar.Tactics.Typeclasses.tcresolve ()] i0: t_Iterator v_I)
+    : t_Iterator (t_Enumerate v_I) =
+  {
+    f_Item = (usize & i0.f_Item);
+    f_next_pre = (fun (self: t_Enumerate v_I) -> true);
+    f_next_post
+    =
+    (fun
+        (self: t_Enumerate v_I)
+        (out1: (t_Enumerate v_I & Core_models.Option.t_Option (usize & i0.f_Item)))
+        ->
+        true);
+    f_next
+    =
+    fun (self: t_Enumerate v_I) ->
+      let (tmp0: v_I), (out: Core_models.Option.t_Option i0.f_Item) =
+        f_next #v_I #FStar.Tactics.Typeclasses.solve self.f_iter
+      in
+      let self:t_Enumerate v_I = { self with f_iter = tmp0 } <: t_Enumerate v_I in
+      let
+      (self: t_Enumerate v_I), (hax_temp_output: Core_models.Option.t_Option (usize & i0.f_Item)) =
+        match out <: Core_models.Option.t_Option i0.f_Item with
+        | Core_models.Option.Option_Some a ->
+          let i:usize = self.f_count in
+          let _:Prims.unit =
+            Hax_lib.v_assume (b2t (self.f_count <. Core_models.Num.impl_usize__MAX <: bool))
+          in
+          let self:t_Enumerate v_I =
+            { self with f_count = self.f_count +! mk_usize 1 } <: t_Enumerate v_I
+          in
+          self,
+          (Core_models.Option.Option_Some (i, a <: (usize & i0.f_Item))
+            <:
+            Core_models.Option.t_Option (usize & i0.f_Item))
+          <:
+          (t_Enumerate v_I & Core_models.Option.t_Option (usize & i0.f_Item))
+        | Core_models.Option.Option_None  ->
+          self, (Core_models.Option.Option_None <: Core_models.Option.t_Option (usize & i0.f_Item))
+          <:
+          (t_Enumerate v_I & Core_models.Option.t_Option (usize & i0.f_Item))
+      in
+      self, hax_temp_output <: (t_Enumerate v_I & Core_models.Option.t_Option (usize & i0.f_Item))
+  }
+
+let impl__new__from__flat_map
+      (#v_I #v_U #v_F: Type0)
+      (#[FStar.Tactics.Typeclasses.tcresolve ()] i0: t_Iterator v_I)
+      (#[FStar.Tactics.Typeclasses.tcresolve ()] i1: t_Iterator v_U)
+      (#[FStar.Tactics.Typeclasses.tcresolve ()]
+          i2:
+          Core_models.Ops.Function.t_FnOnce v_F i0.f_Item)
+      (#_: unit{i2.Core_models.Ops.Function.f_Output == v_U})
+      (it: v_I)
+      (f: v_F)
+    : t_FlatMap v_I v_U v_F =
+  {
+    f_it = it;
+    f_f = f;
+    f_current = Core_models.Option.Option_None <: Core_models.Option.t_Option v_U
+  }
+  <:
+  t_FlatMap v_I v_U v_F
+
+[@@ FStar.Tactics.Typeclasses.tcinstance]
+assume
+val impl_1__from__flat_map':
+    #v_I: Type0 ->
+    #v_U: Type0 ->
+    #v_F: Type0 ->
+    {| i0: t_Iterator v_I |} ->
+    {| i1: t_Iterator v_U |} ->
+    {| i2: Core_models.Ops.Function.t_FnOnce v_F i0.f_Item |} ->
+    #_: unit{i2.Core_models.Ops.Function.f_Output == v_U}
+  -> t_Iterator (t_FlatMap v_I v_U v_F)
+
+unfold
+let impl_1__from__flat_map
+      (#v_I #v_U #v_F: Type0)
+      (#[FStar.Tactics.Typeclasses.tcresolve ()] i0: t_Iterator v_I)
+      (#[FStar.Tactics.Typeclasses.tcresolve ()] i1: t_Iterator v_U)
+      (#[FStar.Tactics.Typeclasses.tcresolve ()]
+          i2:
+          Core_models.Ops.Function.t_FnOnce v_F i0.f_Item)
+      (#_: unit{i2.Core_models.Ops.Function.f_Output == v_U})
+     = impl_1__from__flat_map' #v_I #v_U #v_F #i0 #i1 #i2 #_
+
+noeq
+
+type t_Flatten (v_I: Type0) {| i0: t_Iterator v_I |} {| i1: t_Iterator i0.f_Item |} = {
+  f_it:v_I;
+  f_current:Core_models.Option.t_Option i0.f_Item
+}
+
+let impl__new__from__flatten
+      (#v_I: Type0)
+      (#[FStar.Tactics.Typeclasses.tcresolve ()] i0: t_Iterator v_I)
+      (#[FStar.Tactics.Typeclasses.tcresolve ()] i1: t_Iterator i0.f_Item)
+      (it: v_I)
+    : t_Flatten v_I =
+  { f_it = it; f_current = Core_models.Option.Option_None <: Core_models.Option.t_Option i0.f_Item }
+  <:
+  t_Flatten v_I
+
+[@@ FStar.Tactics.Typeclasses.tcinstance]
+assume
+val impl_1__from__flatten':
+    #v_I: Type0 ->
+    {| i0: t_Iterator v_I |} ->
+    {| i1: t_Iterator i0.f_Item |}
+  -> t_Iterator (t_Flatten v_I)
+
+unfold
+let impl_1__from__flatten
+      (#v_I: Type0)
+      (#[FStar.Tactics.Typeclasses.tcresolve ()] i0: t_Iterator v_I)
+      (#[FStar.Tactics.Typeclasses.tcresolve ()] i1: t_Iterator i0.f_Item)
+     = impl_1__from__flatten' #v_I #i0 #i1
+
+[@@ FStar.Tactics.Typeclasses.tcinstance]
+let impl_1__from__map
+      (#v_I #v_O #v_F: Type0)
+      (#[FStar.Tactics.Typeclasses.tcresolve ()] i0: t_Iterator v_I)
+      (#[FStar.Tactics.Typeclasses.tcresolve ()]
+          i1:
+          Core_models.Ops.Function.t_FnOnce v_F i0.f_Item)
+      (#_: unit{i1.Core_models.Ops.Function.f_Output == v_O})
+    : t_Iterator (t_Map v_I v_F) =
+  {
+    f_Item = v_O;
+    f_next_pre = (fun (self: t_Map v_I v_F) -> true);
+    f_next_post
+    =
+    (fun (self: t_Map v_I v_F) (out1: (t_Map v_I v_F & Core_models.Option.t_Option v_O)) -> true);
+    f_next
+    =
+    fun (self: t_Map v_I v_F) ->
+      let (tmp0: v_I), (out: Core_models.Option.t_Option i0.f_Item) =
+        f_next #v_I #FStar.Tactics.Typeclasses.solve self.f_iter
+      in
+      let self:t_Map v_I v_F = { self with f_iter = tmp0 } <: t_Map v_I v_F in
+      let hax_temp_output:Core_models.Option.t_Option v_O =
+        match out <: Core_models.Option.t_Option i0.f_Item with
+        | Core_models.Option.Option_Some v ->
+          Core_models.Option.Option_Some
+          (Core_models.Ops.Function.f_call_once #v_F
+              #i0.f_Item
+              #FStar.Tactics.Typeclasses.solve
+              self.f_f
+              v)
+          <:
+          Core_models.Option.t_Option v_O
+        | Core_models.Option.Option_None  ->
+          Core_models.Option.Option_None <: Core_models.Option.t_Option v_O
+      in
+      self, hax_temp_output <: (t_Map v_I v_F & Core_models.Option.t_Option v_O)
+  }
+
+[@@ FStar.Tactics.Typeclasses.tcinstance]
+assume
+val impl_1__from__step_by': #v_I: Type0 -> {| i0: t_Iterator v_I |} -> t_Iterator (t_StepBy v_I)
+
+unfold
+let impl_1__from__step_by
+      (#v_I: Type0)
+      (#[FStar.Tactics.Typeclasses.tcresolve ()] i0: t_Iterator v_I)
+     = impl_1__from__step_by' #v_I #i0
+
+[@@ FStar.Tactics.Typeclasses.tcinstance]
+let impl_1__from__take (#v_I: Type0) (#[FStar.Tactics.Typeclasses.tcresolve ()] i0: t_Iterator v_I)
+    : t_Iterator (t_Take v_I) =
+  {
+    f_Item = i0.f_Item;
+    f_next_pre = (fun (self: t_Take v_I) -> true);
+    f_next_post
+    =
+    (fun (self: t_Take v_I) (out1: (t_Take v_I & Core_models.Option.t_Option i0.f_Item)) -> true);
+    f_next
+    =
+    fun (self: t_Take v_I) ->
+      let (self: t_Take v_I), (hax_temp_output: Core_models.Option.t_Option i0.f_Item) =
+        if self.f_n <>. mk_usize 0
+        then
+          let self:t_Take v_I = { self with f_n = self.f_n -! mk_usize 1 } <: t_Take v_I in
+          let (tmp0: v_I), (out: Core_models.Option.t_Option i0.f_Item) =
+            f_next #v_I #FStar.Tactics.Typeclasses.solve self.f_iter
+          in
+          let self:t_Take v_I = { self with f_iter = tmp0 } <: t_Take v_I in
+          self, out <: (t_Take v_I & Core_models.Option.t_Option i0.f_Item)
+        else
+          self, (Core_models.Option.Option_None <: Core_models.Option.t_Option i0.f_Item)
+          <:
+          (t_Take v_I & Core_models.Option.t_Option i0.f_Item)
+      in
+      self, hax_temp_output <: (t_Take v_I & Core_models.Option.t_Option i0.f_Item)
+  }
+
+let impl__new__from__zip
+      (#v_I1 #v_I2: Type0)
+      (#[FStar.Tactics.Typeclasses.tcresolve ()] i0: t_Iterator v_I1)
+      (#[FStar.Tactics.Typeclasses.tcresolve ()] i1: t_Iterator v_I2)
+      (it1: v_I1)
+      (it2: v_I2)
+    : t_Zip v_I1 v_I2 = { f_it1 = it1; f_it2 = it2 } <: t_Zip v_I1 v_I2
+
+[@@ FStar.Tactics.Typeclasses.tcinstance]
+assume
+val impl_1__from__zip':
+    #v_I1: Type0 ->
+    #v_I2: Type0 ->
+    {| i0: t_Iterator v_I1 |} ->
+    {| i1: t_Iterator v_I2 |}
+  -> t_Iterator (t_Zip v_I1 v_I2)
+
+unfold
+let impl_1__from__zip
+      (#v_I1 #v_I2: Type0)
+      (#[FStar.Tactics.Typeclasses.tcresolve ()] i0: t_Iterator v_I1)
+      (#[FStar.Tactics.Typeclasses.tcresolve ()] i1: t_Iterator v_I2)
+     = impl_1__from__zip' #v_I1 #v_I2 #i0 #i1
+
+assume
+val fold':
+    #v_I: Type0 ->
+    #v_B: Type0 ->
+    #v_F: Type0 ->
+    {| i0: t_Iterator v_I |} ->
+    {| i1: Core_models.Ops.Function.t_FnOnce v_F (v_B & i0.f_Item) |} ->
+    #_: unit{i1.Core_models.Ops.Function.f_Output == v_B} ->
+    it: v_I ->
+    init: v_B ->
+    f: v_F
+  -> v_B
+
+unfold
+let fold
+      (#v_I #v_B #v_F: Type0)
+      (#[FStar.Tactics.Typeclasses.tcresolve ()] i0: t_Iterator v_I)
+      (#[FStar.Tactics.Typeclasses.tcresolve ()]
+          i1:
+          Core_models.Ops.Function.t_FnOnce v_F (v_B & i0.f_Item))
+      (#_: unit{i1.Core_models.Ops.Function.f_Output == v_B})
+     = fold' #v_I #v_B #v_F #i0 #i1 #_
+
+let enumerate (#v_I: Type0) (#[FStar.Tactics.Typeclasses.tcresolve ()] i0: t_Iterator v_I) (it: v_I)
+    : t_Enumerate v_I = impl__new #v_I it
+
+let step_by
+      (#v_I: Type0)
+      (#[FStar.Tactics.Typeclasses.tcresolve ()] i0: t_Iterator v_I)
+      (it: v_I)
+      (step: usize)
+    : t_StepBy v_I = impl__new__from__step_by #v_I it step
+
+let map
+      (#v_I #v_O #v_F: Type0)
+      (#[FStar.Tactics.Typeclasses.tcresolve ()] i0: t_Iterator v_I)
+      (#[FStar.Tactics.Typeclasses.tcresolve ()]
+          i1:
+          Core_models.Ops.Function.t_FnOnce v_F i0.f_Item)
+      (#_: unit{i1.Core_models.Ops.Function.f_Output == v_O})
+      (it: v_I)
+      (f: v_F)
+    : t_Map v_I v_F = impl__new__from__map #v_I #v_F it f
+
+assume
+val all':
+    #v_I: Type0 ->
+    #v_F: Type0 ->
+    {| i0: t_Iterator v_I |} ->
+    {| i1: Core_models.Ops.Function.t_FnOnce v_F i0.f_Item |} ->
+    #_: unit{i1.Core_models.Ops.Function.f_Output == bool} ->
+    it: v_I ->
+    f: v_F
+  -> bool
+
+unfold
+let all
+      (#v_I #v_F: Type0)
+      (#[FStar.Tactics.Typeclasses.tcresolve ()] i0: t_Iterator v_I)
+      (#[FStar.Tactics.Typeclasses.tcresolve ()]
+          i1:
+          Core_models.Ops.Function.t_FnOnce v_F i0.f_Item)
+      (#_: unit{i1.Core_models.Ops.Function.f_Output == bool})
+     = all' #v_I #v_F #i0 #i1 #_
+
+let take
+      (#v_I: Type0)
+      (#[FStar.Tactics.Typeclasses.tcresolve ()] i0: t_Iterator v_I)
+      (it: v_I)
+      (n: usize)
+    : t_Take v_I = impl__new__from__take #v_I it n
+
+let flat_map
+      (#v_I #v_U #v_F: Type0)
+      (#[FStar.Tactics.Typeclasses.tcresolve ()] i0: t_Iterator v_I)
+      (#[FStar.Tactics.Typeclasses.tcresolve ()] i1: t_Iterator v_U)
+      (#[FStar.Tactics.Typeclasses.tcresolve ()]
+          i2:
+          Core_models.Ops.Function.t_FnOnce v_F i0.f_Item)
+      (#_: unit{i2.Core_models.Ops.Function.f_Output == v_U})
+      (it: v_I)
+      (f: v_F)
+    : t_FlatMap v_I v_U v_F = impl__new__from__flat_map #v_I #v_U #v_F it f
+
+let flatten
+      (#v_I: Type0)
+      (#[FStar.Tactics.Typeclasses.tcresolve ()] i0: t_Iterator v_I)
+      (#[FStar.Tactics.Typeclasses.tcresolve ()] i1: t_Iterator i0.f_Item)
+      (it: v_I)
+    : t_Flatten v_I = impl__new__from__flatten #v_I it
+
+let zip
+      (#v_I1 #v_I2: Type0)
+      (#[FStar.Tactics.Typeclasses.tcresolve ()] i0: t_Iterator v_I1)
+      (#[FStar.Tactics.Typeclasses.tcresolve ()] i1: t_Iterator v_I2)
+      (it1: v_I1)
+      (it2: v_I2)
+    : t_Zip v_I1 v_I2 = impl__new__from__zip #v_I1 #v_I2 it1 it2
