hax-lib/proof-libs/fstar/core/Std.Io.Impls.fsti
@@ -1,7 +1,7 @@
 module Std.Io.Impls
 #set-options "--fuel 0 --ifuel 1 --z3rlimit 15"
 open FStar.Mul
-open Core_models
+open Rust_primitives
 
 [@@ FStar.Tactics.Typeclasses.tcinstance]
 val impl:Std.Io.t_Read (t_Slice u8)
