hax-lib/proof-libs/fstar/core/Core_models.fst
@@ -2,5 +2,4 @@ module Core_models
 
 include Rust_primitives
 include Core_models.Num
-include Core_models.Iter
 include Rust_primitives.Notations
